emacs weird

trans.v
@@ -57,7 +57,7 @@ Fixpoint  trans_type (w1 l1: Syntax.term False) (tau : source.term) {struct tau}
                                                        let U := (ppair u l) in
                                                        arrow (subseq (ppair (shift 3 w1) l1) U)
  (*compm1_Type starts here*)                        (arrow (store U)
-                         (laters (exist nzero preworld ((* u := 2, l:= 1, v = 0*)
+                         (laters (exist nzero preworld ((* l1 = 3, u := 2, l:= 1, v = 0*)
                                           sigma nattp (*l1 = 4 u := 3, l := 2, v= 1, lv := 0*)
                                           (let u := Syntax.var 3 in
                                               let l := Syntax.var 2 in
@@ -65,6 +65,7 @@ Fixpoint  trans_type (w1 l1: Syntax.term False) (tau : source.term) {struct tau}
                                               let lv := Syntax.var 0 in
                                               let U := ppair u l in
                                               let V := ppair v lv in
+                                              (*u = 4, l = 3, subseq = 2, v = 1, lv = 0*)
                                                     prod (prod (subseq U V) (store V))
                                                      (trans_type v lv tau'))))
                                     )
